Started moving high-level proofs to commonsearch

Graphlib/SearchAlgorithm.lean
@@ -186,6 +186,25 @@ decreasing_by
   apply step_returned_none
 
 
+
+lemma search_recurse_obtain_base_termination_property {state_type : Type} [has_base_search_state g state_type]
+    (goal : V)
+    (priorState : state_type)
+    (search_step : search_step_function g)
+    (termination_metric : state_type → ℕ × ℕ)
+    (decreasing_proof : termination_metric_decreasing_proof goal search_step termination_metric)
+        -- until here all necessary for calling the search_recurse
+    (terminated_with : Bool) -- recursion terminated with
+    (property_after_termination : base_search_state g → Prop):
+      (∀ s : state_type, (search_step goal s).2 = some terminated_with → property_after_termination (has_base_search_state.to_base_state (search_step goal s).1))
+    → 
+      ((search_recurse goal priorState search_step termination_metric decreasing_proof).2 = terminated_with → 
+      property_after_termination (has_base_search_state.to_base_state (search_recurse goal priorState search_step termination_metric decreasing_proof).1)) := by
+      intro property_holds
+      apply search_recurse_obtain_termination_property goal priorState search_step termination_metric decreasing_proof (terminated_with) (fun x => property_after_termination (has_base_search_state.to_base_state x)) -- fun needed to tell lean what the "invariant" is it should apply
+      exact property_holds
+
+
 abbrev invar_carries_over_step 
     {state_type : Type} [has_base_search_state g state_type]
     (goal : V)
@@ -292,95 +311,188 @@ lemma search_recurse_lift_base_invariant
       · use invar_holds_on_base
       · use invar_carries
 
+section
 
-def search_internal {state_type : Type} [has_base_search_state g state_type]
-    (start : V)
-    (goal : V)
-    (start_to_state : V → state_type)
-    (search_step : search_step_function g)
-    (termination_metric : state_type → ℕ × ℕ)
-    (decreasing_proof : termination_metric_decreasing_proof goal search_step termination_metric):
-    state_type × Bool :=
-  search_recurse goal (start_to_state start) search_step termination_metric decreasing_proof
+variable {state_type : Type} [has_base_search_state g state_type]
+variable {start : V}
+variable {goal : V}
+variable {start_state : state_type}
+variable {search_step : search_step_function g (state_type := state_type)}
+variable {termination_metric : state_type → ℕ × ℕ}
 
 
+def search_internal
+  (decreasing_proof : termination_metric_decreasing_proof goal search_step termination_metric):
+  state_type × Bool :=
+  search_recurse goal start_state search_step termination_metric decreasing_proof
 
-abbrev search_visited_goal_if_returned_true {state_type : Type} [has_base_search_state g state_type]
-    (start : V)
-    (goal : V)
-    (start_to_state : V → state_type)
-    (search_step : search_step_function g)
-    (termination_metric : state_type → ℕ × ℕ)
-    (decreasing_proof : termination_metric_decreasing_proof goal search_step termination_metric):=
-    let ret := (search_internal start goal start_to_state search_step termination_metric decreasing_proof)
-    ret.2 = true → goal ∈ (has_base_search_state.to_base_state (g:=g) ret.1).visited
+
+lemma search_returns_with_invariants
+  (decreasing_proof : termination_metric_decreasing_proof goal search_step termination_metric)
+  (start_is_base_init : (has_base_search_state.to_base_state (g:=g) start_state) = (base_search_state_initial start))
+  (invar_carries_over_step : base_invar_carries_over_step goal search_step (search_invar_all_basic start)):
+    search_invar_all_basic start (has_base_search_state.to_base_state (g:=g) (search_internal (start_state:=start_state) decreasing_proof).1) := by
+    unfold search_internal
+    apply search_recurse_lift_base_invariant 
+    constructor
+    · rw [start_is_base_init]
+      unfold base_search_state_initial
+      simp_all
+      apply base_search_state_initial_all_basic_invars
+    · exact invar_carries_over_step
+
+      --unfold base_invar_carries_over_step
+      --intro s cond
+      --apply dfs_step_keeps_all_basic_invars
+      --exact cond
+ 
+lemma search_returns_with_stack_visited
+  (decreasing_proof : termination_metric_decreasing_proof goal search_step termination_metric)
+  (start_is_base_init : (has_base_search_state.to_base_state (g:=g) start_state) = (base_search_state_initial start))
+  (invar_carries_over_step : base_invar_carries_over_step goal search_step (search_invar_all_basic start)):
+    search_invar_stack_is_visited (has_base_search_state.to_base_state (g:=g) (search_internal (start_state:=start_state) decreasing_proof).1) := by
+    have all_invars := search_returns_with_invariants (g:=g) decreasing_proof start_is_base_init invar_carries_over_step
+    unfold search_invar_all_basic at all_invars
+    exact all_invars.1
+
+
+
+abbrev search_step_goal_on_stack_if_terminated :=
+    ∀ s : state_type, ∀ goal : V, (search_step goal s).2 = true →
+      goal ∈ (has_base_search_state.to_base_state (g:=g) (search_step goal s).1).stack 
+
+
+lemma search_goal_on_stack_if_returned_true
+  (decreasing_proof : termination_metric_decreasing_proof goal search_step termination_metric)
+  (goal_on_stack_if_terminated : search_step_goal_on_stack_if_terminated (search_step:=search_step)):
+    (search_internal (g:=g) (start_state:=start_state) decreasing_proof).2 = true →
+      search_prop_goal_on_stack goal (has_base_search_state.to_base_state (g:=g) (search_internal (start_state:=start_state) decreasing_proof).1) := by 
+    intro terminated_with_goal_found 
+    unfold search_internal
+    apply search_recurse_obtain_base_termination_property goal (start_state) (property_after_termination := search_prop_goal_on_stack goal) (terminated_with := true) 
+    · intro s
+      apply goal_on_stack_if_terminated
+    · exact terminated_with_goal_found
+
+
+lemma search_visited_goal_if_returned_true 
+  (decreasing_proof : termination_metric_decreasing_proof goal search_step termination_metric)
+  (start_is_base_init : (has_base_search_state.to_base_state (g:=g) start_state) = (base_search_state_initial start))
+  (invar_carries_over_step : base_invar_carries_over_step goal search_step (search_invar_all_basic start))
+  (goal_on_stack_if_terminated : search_step_goal_on_stack_if_terminated (search_step:=search_step)):
+  (search_internal (g:=g) (start_state:=start_state) decreasing_proof).2 = true → goal ∈ (has_base_search_state.to_base_state (g:=g) (search_internal (start_state:=start_state) decreasing_proof).1).visited := by 
+    intro terminated_with_goal_found 
+    apply search_returns_with_stack_visited 
+    · exact start_is_base_init 
+    · exact invar_carries_over_step
+    · apply search_goal_on_stack_if_returned_true
+      · exact goal_on_stack_if_terminated
+      · exact terminated_with_goal_found 
+
+
+--lemma dfs_returns_with_mother_visited (start : V) (goal : V):
+--    search_invar_mother_is_visited (dfs_internal g start goal).1 := by
+--    have all_invars := dfs_returns_with_invariants g start goal
+--    unfold search_invar_all_basic at all_invars
+--    exact all_invars.2.1
+--
+--lemma dfs_returns_with_mother_adjacent (start : V) (goal : V):
+--    search_invar_mother_is_adjacent start (dfs_internal g start goal).1 := by
+--    have all_invars := dfs_returns_with_invariants g start goal
+--    unfold search_invar_all_basic at all_invars
+--    exact all_invars.2.2.1
+--
+--lemma dfs_returns_with_mother_decreasing (start : V) (goal : V):
+--    search_invar_mother_decreasing_path_order start (dfs_internal g start goal).1 := by
+--    have all_invars := dfs_returns_with_invariants g start goal
+--    unfold search_invar_all_basic at all_invars
+--    exact all_invars.2.2.2.1
+--
+--lemma dfs_returns_with_start_visited (start : V) (goal : V):
+--    search_invar_start_visited start (dfs_internal g start goal).1 := by
+--    have all_invars := dfs_returns_with_invariants g start goal
+--    unfold search_invar_all_basic at all_invars
+--    exact all_invars.2.2.2.2.2
+--
+--lemma dfs_returns_with_node_on_stack_or_all_neighbours_visited (start : V) (goal : V):
+--    search_invar_on_stack_or_all_neighbours_visited (dfs_internal g start goal).1 := by
+--    have all_invars := dfs_returns_with_invariants g start goal
+--    unfold search_invar_all_basic at all_invars
+--    exact all_invars.2.2.2.2.1
+
 
 abbrev search_returns_with_mother_visited {state_type : Type} [has_base_search_state g state_type]
-    (start : V)
     (goal : V)
-    (start_to_state : V → state_type)
+    (start_state : state_type)
     (search_step : search_step_function g)
     (termination_metric : state_type → ℕ × ℕ)
     (decreasing_proof : termination_metric_decreasing_proof goal search_step termination_metric):=
-    search_invar_mother_is_visited (has_base_search_state.to_base_state (g:=g) (search_internal start goal start_to_state search_step termination_metric decreasing_proof).1)
+    search_invar_mother_is_visited (has_base_search_state.to_base_state (g:=g) (search_internal (start_state:=start_state) decreasing_proof).1)
 
 abbrev search_returns_with_mother_adjacent {state_type : Type} [has_base_search_state g state_type]
     (start : V)
     (goal : V)
-    (start_to_state : V → state_type)
+    (start_state : state_type)
     (search_step : search_step_function g)
     (termination_metric : state_type → ℕ × ℕ)
     (decreasing_proof : termination_metric_decreasing_proof goal search_step termination_metric):=
-    search_invar_mother_is_adjacent start (has_base_search_state.to_base_state (g:=g) (search_internal start goal start_to_state search_step termination_metric decreasing_proof).1)
+    search_invar_mother_is_adjacent start (has_base_search_state.to_base_state (g:=g) (search_internal (start_state:=start_state) decreasing_proof).1)
 
 abbrev search_returns_with_mother_decreasing {state_type : Type} [has_base_search_state g state_type]
     (start : V)
     (goal : V)
-    (start_to_state : V → state_type)
+    (start_state : state_type)
     (search_step : search_step_function g)
     (termination_metric : state_type → ℕ × ℕ)
     (decreasing_proof : termination_metric_decreasing_proof goal search_step termination_metric):= 
-    search_invar_mother_decreasing_path_order start (has_base_search_state.to_base_state (g:=g) (search_internal start goal start_to_state search_step termination_metric decreasing_proof).1)
+    search_invar_mother_decreasing_path_order start (has_base_search_state.to_base_state (g:=g) (search_internal (start_state:=start_state) decreasing_proof).1)
 
 
-def search_exe {state_type : Type} [has_base_search_state g state_type]
-    (start : V)
-    (goal : V)
-    (start_to_state : V → state_type)
-    (search_step : search_step_function g)
-    (termination_metric : state_type → ℕ × ℕ)
+def search_exe
     (decreasing_proof : termination_metric_decreasing_proof goal search_step termination_metric)
-    (goal_if_return_true : search_visited_goal_if_returned_true start goal start_to_state search_step termination_metric decreasing_proof)
-    (mother_visited : search_returns_with_mother_visited start goal start_to_state search_step termination_metric decreasing_proof)
-    (mother_adjacent : search_returns_with_mother_adjacent start goal start_to_state search_step termination_metric decreasing_proof)
-    (mother_decreasing : search_returns_with_mother_decreasing start goal start_to_state search_step termination_metric decreasing_proof):
+    (start_is_base_init : (has_base_search_state.to_base_state (g:=g) start_state) = (base_search_state_initial start))
+    (invar_carries_over_step : base_invar_carries_over_step goal search_step (search_invar_all_basic start))
+    (goal_on_stack_if_terminated : search_step_goal_on_stack_if_terminated (search_step:=search_step))
+
+-----
+    (mother_visited : search_returns_with_mother_visited goal start_state search_step termination_metric decreasing_proof)
+    (mother_adjacent : search_returns_with_mother_adjacent start goal start_state search_step termination_metric decreasing_proof)
+    (mother_decreasing : search_returns_with_mother_decreasing start goal start_state search_step termination_metric decreasing_proof):
     Option (Path g start goal) :=
-  let ret := search_internal start goal start_to_state search_step termination_metric decreasing_proof
+  let ret := search_internal decreasing_proof
   let final_state:= ret.1
   let found_goal := ret.2
 
   if found_goal_true : found_goal = true then
+
+    have goal_in_final_visited : goal ∈ (has_base_search_state.to_base_state (g:=g) (search_internal (start_state:=start_state) decreasing_proof).1).visited := by
+      apply search_visited_goal_if_returned_true 
+      · use start_is_base_init
+      · use invar_carries_over_step
+      · use goal_on_stack_if_terminated
+      · use found_goal_true
+
     some (extract_path_to start goal (has_base_search_state.to_base_state final_state)
-      (goal_if_return_true found_goal_true) mother_visited mother_adjacent mother_decreasing).1
+      goal_in_final_visited mother_visited mother_adjacent mother_decreasing).1
   else
     none
 
 theorem search_is_sound {state_type : Type} [has_base_search_state g state_type]
     (start : V)
     (goal : V)
-    (start_to_state : V → state_type)
+    (start_state : state_type)
     (search_step : search_step_function g)
     (termination_metric : state_type → ℕ × ℕ)
     (decreasing_proof : termination_metric_decreasing_proof goal search_step termination_metric)
-    (goal_if_return_true : search_visited_goal_if_returned_true start goal start_to_state search_step termination_metric decreasing_proof)
-    (mother_visited : search_returns_with_mother_visited start goal start_to_state search_step termination_metric decreasing_proof)
-    (mother_adjacent : search_returns_with_mother_adjacent start goal start_to_state search_step termination_metric decreasing_proof)
-    (mother_decreasing : search_returns_with_mother_decreasing start goal start_to_state search_step termination_metric decreasing_proof):
-    (Option.isSome (search_exe start goal start_to_state search_step termination_metric decreasing_proof goal_if_return_true mother_visited mother_adjacent mother_decreasing) → (∃ x : (Path g start goal), x = x)) := by
+    (goal_if_return_true : search_visited_goal_if_returned_true goal start_state search_step termination_metric decreasing_proof)
+    (mother_visited : search_returns_with_mother_visited goal start_state search_step termination_metric decreasing_proof)
+    (mother_adjacent : search_returns_with_mother_adjacent start goal start_state search_step termination_metric decreasing_proof)
+    (mother_decreasing : search_returns_with_mother_decreasing start goal start_state search_step termination_metric decreasing_proof):
+    (Option.isSome (search_exe start goal start_state search_step termination_metric decreasing_proof goal_if_return_true mother_visited mother_adjacent mother_decreasing) → (∃ x : (Path g start goal), x = x)) := by
   intro h -- Option.isSome true on some and false on none, x = x since we need a formula
   constructor -- since goal is existence
   rfl
-  let w := Option.get (search_exe start goal start_to_state search_step termination_metric decreasing_proof goal_if_return_true mother_visited mother_adjacent mother_decreasing) -- Option.get extracts value of returned some and fails otherwise
+  let w := Option.get (search_exe start goal start_state search_step termination_metric decreasing_proof goal_if_return_true mother_visited mother_adjacent mother_decreasing) -- Option.get extracts value of returned some and fails otherwise
   apply w
   simp_all
 
@@ -388,69 +500,66 @@ theorem search_is_sound {state_type : Type} [has_base_search_state g state_type]
 abbrev search_returns_with_start_visited {state_type : Type} [has_base_search_state g state_type]
     (start : V)
     (goal : V)
-    (start_to_state : V → state_type)
+    (start_state : state_type)
     (search_step : search_step_function g)
     (termination_metric : state_type → ℕ × ℕ)
     (decreasing_proof : termination_metric_decreasing_proof goal search_step termination_metric):=
-    search_invar_start_visited start (has_base_search_state.to_base_state (g:=g) (search_internal start goal start_to_state search_step termination_metric decreasing_proof).1)
+    search_invar_start_visited start (has_base_search_state.to_base_state (g:=g) (search_internal goal start_state search_step termination_metric decreasing_proof).1)
 
 abbrev search_returns_with_node_on_stack_or_all_neighbours_visited {state_type : Type} [has_base_search_state g state_type]
-    (start : V)
     (goal : V)
-    (start_to_state : V → state_type)
+    (start_state : state_type)
     (search_step : search_step_function g)
     (termination_metric : state_type → ℕ × ℕ)
     (decreasing_proof : termination_metric_decreasing_proof goal search_step termination_metric):=
-    search_invar_on_stack_or_all_neighbours_visited (has_base_search_state.to_base_state (g:=g) (search_internal start goal start_to_state search_step termination_metric decreasing_proof).1)
+    search_invar_on_stack_or_all_neighbours_visited (has_base_search_state.to_base_state (g:=g) (search_internal goal start_state search_step termination_metric decreasing_proof).1)
 
 abbrev search_empty_stack_if_returned_false{state_type : Type} [has_base_search_state g state_type]
-    (start : V)
     (goal : V)
-    (start_to_state : V → state_type)
+    (start_state : state_type)
     (search_step : search_step_function g)
     (termination_metric : state_type → ℕ × ℕ)
     (decreasing_proof : termination_metric_decreasing_proof goal search_step termination_metric)
 :=
-    (search_internal start goal start_to_state search_step termination_metric decreasing_proof).2 = false → (has_base_search_state.to_base_state (g:=g) (search_internal start goal start_to_state search_step termination_metric decreasing_proof).1).stack = [] 
+    (search_internal goal start_state search_step termination_metric decreasing_proof).2 = false → (has_base_search_state.to_base_state (g:=g) (search_internal goal start_state search_step termination_metric decreasing_proof).1).stack = [] 
 
 
 abbrev search_not_visited_goal_if_returned_false{state_type : Type} [has_base_search_state g state_type]
-    (start : V)
     (goal : V)
-    (start_to_state : V → state_type)
+    (start_state : state_type)
     (search_step : search_step_function g)
     (termination_metric : state_type → ℕ × ℕ)
     (decreasing_proof : termination_metric_decreasing_proof goal search_step termination_metric)
     :=
-    (search_internal start goal start_to_state search_step termination_metric decreasing_proof).2 = false → goal ∉ (has_base_search_state.to_base_state (g:=g) (search_internal start goal start_to_state search_step termination_metric decreasing_proof).1).visited
+    (search_internal goal start_state search_step termination_metric decreasing_proof).2 = false → goal ∉ (has_base_search_state.to_base_state (g:=g) (search_internal goal start_state search_step termination_metric decreasing_proof).1).visited
 
 
 theorem search_is_complete {state_type : Type} [has_base_search_state g state_type]
     (start : V)
     (goal : V)
-    (start_to_state : V → state_type)
+    (start_state : state_type)
     (search_step : search_step_function g)
     (termination_metric : state_type → ℕ × ℕ)
     (decreasing_proof : termination_metric_decreasing_proof goal search_step termination_metric)
-    (goal_if_return_true : search_visited_goal_if_returned_true start goal start_to_state search_step termination_metric decreasing_proof)
-    (mother_visited : search_returns_with_mother_visited start goal start_to_state search_step termination_metric decreasing_proof)
-    (mother_adjacent : search_returns_with_mother_adjacent start goal start_to_state search_step termination_metric decreasing_proof)
-    (mother_decreasing : search_returns_with_mother_decreasing start goal start_to_state search_step termination_metric decreasing_proof)
-    (start_visited : search_returns_with_start_visited start goal start_to_state search_step termination_metric decreasing_proof)
-    (on_stack_or_all_nei_visited : search_returns_with_node_on_stack_or_all_neighbours_visited start goal start_to_state search_step termination_metric decreasing_proof)
-    (stack_empty_if_returned_false : search_empty_stack_if_returned_false start goal start_to_state search_step termination_metric decreasing_proof)
-    (goal_not_visited_if_returned_false : search_not_visited_goal_if_returned_false start goal start_to_state search_step termination_metric decreasing_proof):
-    ((∃ x : (Path g start goal), x = x) → Option.isSome (search_exe start goal start_to_state search_step termination_metric decreasing_proof goal_if_return_true mother_visited mother_adjacent mother_decreasing)) := by
+    (goal_if_return_true : search_visited_goal_if_returned_true goal start_state search_step termination_metric decreasing_proof)
+    (mother_visited : search_returns_with_mother_visited goal start_state search_step termination_metric decreasing_proof)
+    (mother_adjacent : search_returns_with_mother_adjacent start goal start_state search_step termination_metric decreasing_proof)
+    (mother_decreasing : search_returns_with_mother_decreasing start goal start_state search_step termination_metric decreasing_proof)
+    (start_visited : search_returns_with_start_visited start goal start_state search_step termination_metric decreasing_proof)
+    (on_stack_or_all_nei_visited : search_returns_with_node_on_stack_or_all_neighbours_visited goal start_state search_step termination_metric decreasing_proof)
+    (stack_empty_if_returned_false : search_empty_stack_if_returned_false goal start_state search_step termination_metric decreasing_proof)
+    (goal_not_visited_if_returned_false : search_not_visited_goal_if_returned_false goal start_state search_step termination_metric decreasing_proof):
+    ((∃ x : (Path g start goal), x = x) → Option.isSome (search_exe start goal start_state search_step termination_metric decreasing_proof goal_if_return_true mother_visited mother_adjacent mother_decreasing)) := by
     -- or Option.isNone (dfs g start goal) → ∄ x (Path g start goal), x = x
       intro path_exists
       apply Exists.elim path_exists
       intro thePath a; clear a-- uninformativ x=X
 
-      let final := search_internal start goal start_to_state search_step termination_metric decreasing_proof
+      let final := search_internal goal start_state search_step termination_metric decreasing_proof
       let final_state : base_search_state g := has_base_search_state.to_base_state final.1
       
       --have start_visited : search_invar_start_visited start final_state :=
-      --  search_returns_with_start_visited start goal start_to_state search_step termination_metric decreasing_proof goal_if_return_true mother_visited mother_adjacent mother_decreasing
+      --  search_returns_with_start_visited start goal start_state search_step termination_metric decreasing_proof goal_if_return_true mother_visited mother_adjacent mother_decreasing
       --have on_stack_or_all_nei_visited : search_invar_on_stack_or_all_neighbours_visited final_state:=
       --  dfs_returns_with_node_on_stack_or_all_neighbours_visited start goal
 
@@ -458,7 +567,7 @@ theorem search_is_complete {state_type : Type} [has_base_search_state g state_ty
       by_contra terminates_with_none
       simp at terminates_with_none
 
-      have dfs_returned_false : (search_internal start goal start_to_state search_step termination_metric decreasing_proof).2 = false := by
+      have dfs_returned_false : (search_internal goal start_state search_step termination_metric decreasing_proof).2 = false := by
         unfold search_exe at terminates_with_none
         simp at terminates_with_none
         exact terminates_with_none
@@ -475,20 +584,22 @@ theorem search_is_complete {state_type : Type} [has_base_search_state g state_ty
 theorem search_is_complete_inv  {state_type : Type} [has_base_search_state g state_type]
     (start : V)
     (goal : V)
-    (start_to_state : V → state_type)
+    (start_state : state_type)
     (search_step : search_step_function g)
     (termination_metric : state_type → ℕ × ℕ)
     (decreasing_proof : termination_metric_decreasing_proof goal search_step termination_metric)
-    (goal_if_return_true : search_visited_goal_if_returned_true start goal start_to_state search_step termination_metric decreasing_proof)
-    (mother_visited : search_returns_with_mother_visited start goal start_to_state search_step termination_metric decreasing_proof)
-    (mother_adjacent : search_returns_with_mother_adjacent start goal start_to_state search_step termination_metric decreasing_proof)
-    (mother_decreasing : search_returns_with_mother_decreasing start goal start_to_state search_step termination_metric decreasing_proof)
-    (start_visited : search_returns_with_start_visited start goal start_to_state search_step termination_metric decreasing_proof)
-    (on_stack_or_all_nei_visited : search_returns_with_node_on_stack_or_all_neighbours_visited start goal start_to_state search_step termination_metric decreasing_proof)
-    (stack_empty_if_returned_false : search_empty_stack_if_returned_false start goal start_to_state search_step termination_metric decreasing_proof)
-    (goal_not_visited_if_returned_false : search_not_visited_goal_if_returned_false start goal start_to_state search_step termination_metric decreasing_proof):
-    Option.isNone (search_exe start goal start_to_state search_step termination_metric decreasing_proof goal_if_return_true mother_visited mother_adjacent mother_decreasing) → ¬ ∃ x : (Path g start goal), x = x := by
+    (goal_if_return_true : search_visited_goal_if_returned_true goal start_state search_step termination_metric decreasing_proof)
+    (mother_visited : search_returns_with_mother_visited goal start_state search_step termination_metric decreasing_proof)
+    (mother_adjacent : search_returns_with_mother_adjacent start goal start_state search_step termination_metric decreasing_proof)
+    (mother_decreasing : search_returns_with_mother_decreasing start goal start_state search_step termination_metric decreasing_proof)
+    (start_visited : search_returns_with_start_visited start goal start_state search_step termination_metric decreasing_proof)
+    (on_stack_or_all_nei_visited : search_returns_with_node_on_stack_or_all_neighbours_visited goal start_state search_step termination_metric decreasing_proof)
+    (stack_empty_if_returned_false : search_empty_stack_if_returned_false goal start_state search_step termination_metric decreasing_proof)
+    (goal_not_visited_if_returned_false : search_not_visited_goal_if_returned_false goal start_state search_step termination_metric decreasing_proof):
+    Option.isNone (search_exe start goal start_state search_step termination_metric decreasing_proof goal_if_return_true mother_visited mother_adjacent mother_decreasing) → ¬ ∃ x : (Path g start goal), x = x := by
       intro optionIsNone
       by_contra pathExists
-      have isSome := search_is_complete start goal start_to_state search_step termination_metric decreasing_proof goal_if_return_true mother_visited mother_adjacent mother_decreasing start_visited on_stack_or_all_nei_visited stack_empty_if_returned_false goal_not_visited_if_returned_false
+      have isSome := search_is_complete start goal start_state search_step termination_metric decreasing_proof goal_if_return_true mother_visited mother_adjacent mother_decreasing start_visited on_stack_or_all_nei_visited stack_empty_if_returned_false goal_not_visited_if_returned_false
       simp_all
+
+end
